soundness for evaluator (not complete, there may be a bug. cf. Maybe example)

SystemFD/Evaluator/SmallStep.lean
@@ -6,73 +6,220 @@ set_option maxHeartbeats 400000
 
 
 @[simp]
-def eval_choice_mapping : (t : Term) -> Option Term
+def eval_choice_mapping (Γ : Ctx Term): (t : Term) -> Option Term
 | .ite p (.ctor2 .choice s1 s2) i t => .some (.ite p s1 i t ⊕ .ite p s2 i t)
+| .ite p s i t => do
+   let s' <- eval_choice_mapping Γ s
+   .some (.ite p s' i t)
+
 | .guard p (.ctor2 .choice s1 s2) i => .some (.guard p s1 i ⊕ .guard p s2 i)
+| .guard p s i => do
+   let s' <- eval_choice_mapping Γ s
+   .some (.guard p s' i)
 
 | .ctor1 v (.ctor2 .choice t1 t2) => .some (.ctor2 .choice (.ctor1 v t1) (.ctor1 v t2))
+| .ctor1 v t => do
+  let t' <- eval_choice_mapping Γ t
+  .some (.ctor1 v t')
 
 | .ctor2 .cast f (.ctor2 .choice a1 a2) => .some (.ctor2 .choice (.ctor2 .cast f a1) (.ctor2 .cast f a2))
-| .ctor2 .fst f (.ctor2 .choice a1 a2) => .some (.ctor2 .choice (.ctor2 .fst f a1) (.ctor2 .fst f a2))
-| .ctor2 .snd f (.ctor2 .choice a1 a2) => .some (.ctor2 .choice (.ctor2 .snd f a1) (.ctor2 .snd f a2))
+| .ctor2 .cast t η => do
+  let η' <- eval_choice_mapping Γ η
+  .some (t ▹ η')
 
-| .ctor2 v (.ctor2 .choice f1 f2) a => .some (.ctor2 .choice (.ctor2 v f1 a) (.ctor2 v f2 a))
+| .ctor2 .fst f (.ctor2 .choice a1 a2) => .some (.ctor2 .choice (.ctor2 .fst f a1) (.ctor2 .fst f a2))
+| .ctor2 .fst K η => do
+   let η' <- eval_choice_mapping Γ η
+   .some (fst! K η')
+
+| .ctor2 .snd f (.ctor2 .choice a1 a2) => .some (.ctor2 .choice (.ctor2 .snd f a1) (.ctor2 .snd f a2))
+| .ctor2 .snd K1 η => do
+   let η' <- eval_choice_mapping Γ η
+   .some (snd! K1 η')
+
+| .ctor2 .choice t1 t2 => -- for now, go left to right on choice
+  match eval_choice_mapping Γ t1 with
+  | .some t1' => .some (t1' ⊕ t2)
+  | .none => match eval_choice_mapping Γ t2 with
+             | .some t2' => .some (t1 ⊕ t2')
+             | .none => .none
+
+| .ctor2 v (.ctor2 .choice f1 f2) a =>
+  if v == .choice -- Do not distribute choice over choice (causes infinite loopiness)
+  then .none
+  else if ctor2_has_congr1 v
+       then .some (.ctor2 .choice (.ctor2 v f1 a) (.ctor2 v f2 a))
+       else .none
 
 | .bind2 .arrowc (.ctor2 .choice t1 t2) a => .some (.ctor2 .choice (.bind2 .arrowc t1 a) (.bind2 .arrowc t2 a))
-| .bind2 .allc t (.ctor2 .choice a1 a2) => .some (.ctor2 .choice (.bind2 .allc t a1) (.bind2 .arrowc t a2))
+| .bind2 .arrowc t η => do
+  let η' <- eval_choice_mapping (.empty :: Γ) η
+  .some (.bind2 .arrowc t η')
 
--- TODO: recurse downwards
+| .bind2 .allc t (.ctor2 .choice a1 a2) => .some (.ctor2 .choice (.bind2 .allc t a1) (.bind2 .allc t a2))
+| .bind2 .allc t η => do
+  let η' <- eval_choice_mapping (.kind t :: Γ) η
+  .some (∀c[t] η')
 
 | _ => .none
 
+
 @[simp]
-def eval_const_folding : (t : Term) -> Option Term
--- | .letterm _ t `0 => .some `0
+def eval_const_folding1 (Γ : Ctx Term) : (t : Term) -> Option Term
 | .ite _ `0 _ _ => .some `0
+| .ite p s i t => do
+   let s' <- eval_const_folding1 Γ s
+   .some (.ite p s' i t)
+
 | .guard _ `0 _ => .some `0
+| .guard p s i => do
+   let s' <- eval_const_folding1 Γ s
+   .some (.guard p s' i)
 
 | .ctor1 _ `0 => .some `0
-| .ctor1 _ (.ctor2 .refl K t) => .some (refl! K t)
+| .ctor1 v t => do
+  let t' <- eval_const_folding1 Γ t
+  .some (.ctor1 v t')
 
 | .ctor2 .choice `0 t2 => .some t2
 | .ctor2 .choice t1 `0 => .some t1
 
 | .ctor2 .cast _ `0 => .some `0
-| .ctor2 .cast t (.ctor2 .refl _ _) => .some t
+| .ctor2 .cast t η => do
+  let η' <- eval_const_folding1 Γ η
+  .some (t ▹ η')
 
 | .ctor2 .fst _ `0 => .some `0
-| .ctor2 .fst K1 (.ctor2 .refl K2 (.ctor2 .appk A _)) =>
-  .some (refl! (K1 -k> K2) A)
+| .ctor2 .fst K η => do
+   let η' <- eval_const_folding1 Γ η
+   .some (fst! K η')
 
 | .ctor2 .snd _ `0 => .some `0
-| .ctor2 .snd K1 (.ctor2 .refl _ (.ctor2 .appk _ B)) =>
-  .some (refl! K1 B)
+| .ctor2 .snd K1 η => do
+   let η' <- eval_const_folding1 Γ η
+   .some (snd! K1 η')
 
-| .ctor2 _ `0 _ => .some `0
+| .ctor2 v `0 _ => if ctor2_has_congr1 v then .some `0 else .none
+-- | .ctor2 _ _ `0 => .some `0 -- TODO?
 
-| .ctor2 .seq (.ctor2 .refl K t) (.ctor2 .refl K' t') =>
-  if t == t' && K == K' -- matched during type checking?
-  then .some (refl! K t) else .none
+| .ctor2 .choice t1 t2 => -- for now, go left to right on choice
+  match eval_const_folding1 Γ t1 with
+  | .some t1' => .some (t1' ⊕ t2)
+  | .none => match eval_const_folding1 Γ t2 with
+             | .some t2' => .some (t1 ⊕ t2')
+             | .none => .none
 
-| .ctor2 .appc (.ctor2 .refl (K1 -k> K) t) (.ctor2 .refl K2 t') =>
-  if K1 == K2  -- ideally argument kinds match, but thats done by type checker
-  then .some (refl! K (t `@k t'))  else .none
+| .ctor2 v η1 η2 => if ctor2_has_congr1 v
+  then match eval_const_folding1 Γ η1 with
+       | .some η1' => .some (.ctor2 v η1' η2)
+       | .none => if ctor2_has_congr2 v
+                  then match eval_const_folding1 Γ η2 with
+                       | .some η2' => .some (.ctor2 v η1 η2')
+                       | .none => .none
+                  else .none
+  else (if ctor2_has_congr2 v
+       then match eval_const_folding1 Γ η2 with
+           | .some η2' => .some (.ctor2 v η1 η2')
+           | .none => .none
+       else .none)
 
-| .ctor2 .apptc (.ctor2 .refl K1 (.bind2 .all K2 t1)) (.ctor2 .refl K2' t2) =>
-  if K2 == K2' then .some (refl! K1 (t1 β[t2])) else .none
 
 | .bind2 .arrowc `0 _ => .some `0
-| .bind2 .arrowc (.ctor2 .refl ★ t) (.ctor2 .refl ★ t') => .some (refl! ★ (t -t> t'))
+| .bind2 .arrowc t η => do
+  let η' <- eval_const_folding1 (.empty :: Γ) η
+  .some (.bind2 .arrowc t η')
 
 | .bind2 .allc _ `0 => .some `0
-| .bind2 .allc t (.ctor2 .refl K t') => .some (refl! K (∀[t] t'))
-
--- TODO: recurse downwards
+| .bind2 .allc t η => do
+  let η' <- eval_const_folding1 (.kind t :: Γ) η
+  .some (∀c[t] η')
 
 | _ => .none
 
--- set_option diagnostics true
--- set_option diagnostics.threshold 10
+@[simp]
+def eval_const_folding2 (Γ : Ctx Term) : (t : Term) -> Option Term
+| .ite p s i t => do
+  let s' <- eval_const_folding2 Γ s
+  .some (.ite p s' i t)
+| .guard p s i => do
+  let s' <- eval_const_folding2 Γ s
+  .some (.guard p s' i)
+
+| .ctor1 _ (.ctor2 .refl K t) => .some (refl! K t)
+| .ctor1 v η => do
+  let η' <- eval_const_folding2 Γ η
+  .some (.ctor1 v η')
+
+| .ctor2 .cast t (.ctor2 .refl _ _) => .some t
+| .ctor2 .cast t η => do
+  let η' <- eval_const_folding2 Γ η
+  .some (t ▹ η')
+
+| .ctor2 .fst K1 (.ctor2 .refl K2 (.ctor2 .appk A _)) => .some (refl! (K1 -k> K2) A)
+| .ctor2 .fst K η => do
+   let η' <- eval_const_folding2 Γ η
+   .some (fst! K η')
+
+| .ctor2 .snd K1 (.ctor2 .refl _ (.ctor2 .appk _ B)) => .some (refl! K1 B)
+| .ctor2 .snd K1 η => do
+   let η' <- eval_const_folding2 Γ η
+   .some (snd! K1 η')
+
+| .ctor2 .seq (.ctor2 .refl K t) (.ctor2 .refl K' t') =>
+  if K == K' && t == t' then .some (refl! K t) else .none
+| .ctor2 .seq (.ctor2 .refl K t) η2 => do
+   let η2' <- eval_const_folding2 Γ η2
+   .some (.ctor2 .seq (.ctor2 .refl K t) η2')
+
+| .ctor2 .appc (.ctor2 .refl (K1 -k> K) t) (.ctor2 .refl K2 t') =>
+  if K1 == K2 then .some (refl! K (t `@k t')) else .none
+| .ctor2 .appc (.ctor2 .refl K t) η2 => do
+   let η2' <- eval_const_folding2 Γ η2
+   .some (.ctor2 .appc (.ctor2 .refl K t) η2')
+
+| .ctor2 .apptc (.ctor2 .refl K1 (.bind2 .all K2 t1)) (.ctor2 .refl K2' t2) =>
+  if K2 == K2' then .some (refl! K1 (t1 β[t2])) else .none
+| .ctor2 .apptc (.ctor2 .refl K t) η2 => do
+   let η2' <- eval_const_folding2 Γ η2
+   .some (.ctor2 .apptc (.ctor2 .refl K t) η2')
+
+| .ctor2 .choice t1 t2 => -- for now, go left to right on choice
+  match eval_const_folding2 Γ t1 with
+  | .some t1' => .some (t1' ⊕ t2)
+  | .none => match eval_const_folding2 Γ t2 with
+             | .some t2' => .some (t1 ⊕ t2')
+             | .none => .none
+
+| .ctor2 v η1 η2 =>
+  if ctor2_has_congr1 v
+  then match eval_const_folding2 Γ η1 with
+       | .some η1' => .some (.ctor2 v η1' η2)
+       | .none => if ctor2_has_congr2 v
+                  then match eval_const_folding2 Γ η2 with
+                       | .some η2' => .some (.ctor2 v η1 η2')
+                       | .none => .none
+                  else .none
+  else (if ctor2_has_congr2 v
+       then match eval_const_folding2 Γ η2 with
+           | .some η2' => .some (.ctor2 v η1 η2')
+           | .none => .none
+       else .none)
+
+| .bind2 .arrowc (.ctor2 .refl ★ t) (.ctor2 .refl ★ t') => .some (refl! ★ (t -t> t'))
+| .bind2 .arrowc t η => do
+  let η' <- eval_const_folding2 (.empty :: Γ) η
+  .some (.bind2 .arrowc t η')
+
+
+| .bind2 .allc t (.ctor2 .refl K t') => .some (refl! K (∀[t] t'))
+| .bind2 .allc t η => do
+  let η' <- eval_const_folding2 (.kind t :: Γ) η
+  .some (∀c[t] η')
+
+| _ => .none
+
+
+
 -- Instantiates instances/performs a one step term evaluation
 @[simp]
 def eval_inst (Γ : Ctx Term) : (t : Term) -> Option Term
@@ -148,9 +295,6 @@ def eval_inst (Γ : Ctx Term) : (t : Term) -> Option Term
 --- Ctors1
 ---------------------------
 
--- | .ctor1 _ `0 => .some `0
--- | .ctor1 v (.ctor2 .choice t1 t2) => .some (.ctor2 .choice (.ctor1 v t1) (.ctor1 v t2))
--- | .ctor1 _ (.ctor2 .refl K t) => .some (refl! K t)
 | .ctor1 v η => do
   let η' <- eval_inst Γ η
   .some (.ctor1 v η')
@@ -159,46 +303,25 @@ def eval_inst (Γ : Ctx Term) : (t : Term) -> Option Term
 --- Ctors2
 ---------------------------
 
--- | .ctor2 .choice `0 t2 => .some t2
--- | .ctor2 .choice t1 `0 => .some t1
--- | .ctor2 .choice t1 t2 => -- for now, go left to right on choice
---   match eval_inst Γ t1 with
---   | .some t1' => .some (t1' ⊕ t2)
---   | .none => match eval_inst Γ t2 with
---              | .some t2' => .some (t1 ⊕ t2')
---              | .none => .none
-
---- Evaluate second component first
--- | .ctor2 .cast t (.ctor2 .refl _ _) => .some t
--- | .ctor2 .cast _ `0 => .some `0
--- | .ctor2 .cast f (.ctor2 .choice a1 a2) => .some (.ctor2 .choice (.ctor2 .cast f a1) (.ctor2 .cast f a2))
 | .ctor2 .cast t η => do
   let η' <- eval_inst Γ η
   .some (t ▹ η')
 
--- | .ctor2 .fst K1 (.ctor2 .refl K2 (.ctor2 .appk A _)) =>
---   .some (refl! (K1 -k> K2) A)
--- | .ctor2 .fst _ `0 => .some `0
--- | .ctor2 .fst f (.ctor2 .choice a1 a2) => .some (.ctor2 .choice (.ctor2 .fst f a1) (.ctor2 .fst f a2))
 | .ctor2 .fst K η => do
    let η' <- eval_inst Γ η
    .some (fst! K η')
 
--- | .ctor2 .snd K1 (.ctor2 .refl _ (.ctor2 .appk _ B)) =>
---   .some (refl! K1 B)
--- | .ctor2 .snd _ `0 => .some `0
--- | .ctor2 .snd f (.ctor2 .choice a1 a2) => .some (.ctor2 .choice (.ctor2 .snd f a1) (.ctor2 .snd f a2))
 | .ctor2 .snd K1 η => do
    let η' <- eval_inst Γ η
    .some (snd! K1 η')
 
---- Evaluate first component first
--- | .ctor2 _ `0 _ => .some `0
--- | .ctor2 v (.ctor2 .choice f1 f2) a => .some (.ctor2 .choice (.ctor2 v f1 a) (.ctor2 v f2 a))
-
 | .ctor2 .app (.bind2 .lam _ b) t => .some (b β[ t ])
 | .ctor2 .app f t =>
   match f.neutral_form with
+  | .none => do
+      let f' <- eval_inst Γ f
+      .some (f' `@ t) -- call by name
+
   | .some (h, sp) =>
     (match (Γ d@ h) with
       | .openm _ =>
@@ -207,9 +330,6 @@ def eval_inst (Γ : Ctx Term) : (t : Term) -> Option Term
         .some (List.foldl (·⊕·) `0 ts `@ t)
       | .term _ b => .some ((b.apply_spine sp) `@ t)  -- inline a let bound term
       | _ => .none ) -- nothing to evaluate to
-  | .none => do
-      let f' <- eval_inst Γ f
-      .some (f' `@ t) -- call by name
 
 | .ctor2 .appt (.bind2 .lamt _ b) t => .some (b β[ t ])
 | .ctor2 .appt f t =>
@@ -227,46 +347,36 @@ def eval_inst (Γ : Ctx Term) : (t : Term) -> Option Term
       let f' <- eval_inst Γ f
       .some (f' `@t t) -- call by name
 
--- | .ctor2 .seq (.ctor2 .refl K t) (.ctor2 .refl K' t') =>
---   if t == t' && K == K' -- matched during type checking?
---   then .some (refl! K t) else .none
 | .ctor2 .seq (.ctor2 .refl K t) η2 => do
   let η2' <- eval_inst Γ η2
   .some (refl! K t `; η2')
--- | .ctor2 .seq η1 η2 => do
---   let η1' <- eval_inst Γ η1
---   .some (η1' `; η2)
 
--- | .ctor2 .appc (.ctor2 .refl (K1 -k> K) t) (.ctor2 .refl K2 t') =>
---   if K1 == K2  -- ideally argument kinds match, but thats done by type checker
---   then .some (refl! K (t `@k t'))  else .none
 | .ctor2 .appc (.ctor2 .refl K t) η2 => do
   let η2' <- eval_inst Γ η2
   .some ((.ctor2 .refl K t) `@c η2')
--- | .ctor2 .appc η1 η2 => do
---   let η1' <- eval_inst Γ η1
---   .some (η1' `@c η2)
 
--- | .ctor2 .apptc (.ctor2 .refl K1 (.bind2 .all K2 t1)) (.ctor2 .refl K2' t2) =>
---   if K2 == K2' then .some (refl! K1 (t1 β[t2])) else .none
 | .ctor2 .apptc η1 (.ctor2 .refl K t) => do
   let η1' <- eval_inst Γ η1
   .some (η1' `@c[refl! K t])
--- | .ctor2 .apptc η1 η2 => do
---   let η2' <- eval_inst Γ η2
---   .some (η1 `@c[ η2' ])
 
-| .ctor2 v t1 t2 => do
-  let t1' <- eval_inst Γ t1
-  .some (.ctor2 v t1' t2)
+| .ctor2 v η1 η2 => if ctor2_has_congr1 v
+  then match eval_inst Γ η1 with
+       | .some η1' => .some (.ctor2 v η1' η2)
+       | .none => if ctor2_has_congr2 v
+                  then match eval_inst Γ η2 with
+                       | .some η2' => .some (.ctor2 v η1 η2')
+                       | .none => .none
+                  else .none
+  else (if ctor2_has_congr2 v
+       then match eval_inst Γ η2 with
+           | .some η2' => .some (.ctor2 v η1 η2')
+           | .none => .none
+       else .none)
 
 --------------------------
 --- Binders
 ---------------------------
 -- Evaluate first component first
--- | .bind2 .arrowc (.ctor2 .refl ★ t) (.ctor2 .refl ★ t') => .some (refl! ★ (t -t> t'))
--- | .bind2 .arrowc `0 _ => .some `0
--- | .bind2 .arrowc (.ctor2 .choice t1 t2) a => .some (.ctor2 .choice (.bind2 .arrowc t1 a) (.bind2 .arrowc t2 a))
 | .bind2 .arrowc (.ctor2 .refl ★ t) η => do
   let η' <- eval_inst (.empty :: Γ) η
   .some ((refl! ★ t) -c> η')
@@ -276,9 +386,6 @@ def eval_inst (Γ : Ctx Term) : (t : Term) -> Option Term
 
 
 -- Evaluate second component first
--- | .bind2 .allc t (.ctor2 .refl K t') => .some (refl! K (∀[t] t'))
--- | .bind2 .allc _ `0 => .some `0
--- | .bind2 .allc t (.ctor2 .choice a1 a2) => .some (.ctor2 .choice (.bind2 .allc t a1) (.bind2 .arrowc t a2))
 | .bind2 .allc t η => do
   let η' <- eval_inst (.kind t :: Γ) η
   .some (∀c[t] η')
@@ -288,10 +395,12 @@ def eval_inst (Γ : Ctx Term) : (t : Term) -> Option Term
 
 
 def eval_small_step (Γ : Ctx Term) (t : Term) : Option Term :=
-  match eval_choice_mapping t with
+  match eval_choice_mapping Γ t with
   | .some t' => .some t'
-  | .none => match eval_const_folding t with
+  | .none => match eval_const_folding1 Γ t with
              | .some t' => .some t'
-             | .none    => match eval_inst Γ t with
+             | .none    => match eval_const_folding2 Γ t with
                            | .some t' => .some t'
-                           | .none => .none
+                           | .none   => match eval_inst Γ t with
+                                        | .some t' => .some t'
+                                        | .none => .none
