SystemFD/Evaluator/Soundness.lean
@@ -1,351 +1,597 @@
 import SystemFD.Term
+import SystemFD.Term.Equality
 import SystemFD.Reduction
 import SystemFD.Ctx
 import SystemFD.Judgment
 import SystemFD.Evaluator.SmallStep
 
 set_option maxHeartbeats 5000000
-set_option diagnostics true
+-- set_option diagnostics true
 
-theorem eval_inst_soundess : eval_inst Γ t = .some ts -> Red Γ t ts := by
-intro et
-induction Γ, t using eval_inst.induct generalizing ts
-all_goals try (unfold eval_inst at et)
--- case _ Γ n _ om et =>
---   simp_all; subst et;
---   generalize instsp : get_instances Γ n = insts at *;
---   have nfh := @Term.var_neutral_form n; symm at nfh;
---   symm at instsp;
---   apply Red.inst nfh _ instsp; unfold Term.apply_spine; simp_all;
---   apply instsp; rfl
---   simp; rw[om]; unfold Frame.is_openm; simp
 
--- case _ Γ n _ _ lt et =>
---     simp at et; rw [lt] at et; simp at et; subst et;
---     have nf :=  @Term.var_neutral_form n; symm at nf; symm at lt;
---     apply Red.letterm nf lt;
--- case _ et => simp at et
--- case _ et => simp at et; subst et; apply Red.beta
--- case _ et => simp at et; subst et; apply Red.betat
--- case _ Γ _ _ _ et => simp at et; subst et; apply Red.letbeta
+theorem eval_choice_mapping_soudness : eval_choice_mapping Γ t = .some t' -> Red Γ t t' := by
+intro et;
+induction Γ, t using eval_choice_mapping.induct generalizing t'
+all_goals (simp at et)
+all_goals try (rw[<-et])
+all_goals try (
+case _ ih1 =>
+  rw[Option.bind_eq_some] at et;
+  cases et; case _ et =>
+  cases et; case _ h1 et =>
+  cases et;
+  replace h1 := ih1 h1
+  apply Red.bind2_congr2; simp; assumption
+)
+all_goals try (
+case _ ih1 =>
+  rw[Option.bind_eq_some] at et;
+  cases et; case _ et =>
+  cases et; case _ h1 et =>
+  cases et;
+  replace h1 := ih1 h1
+  apply Red.ctor2_congr2; simp; assumption
+)
 
--- case _ Γ f t e n sp fnf t' om et => -- app openm
---   simp at et; rw[fnf] at et; simp at et; rw[om] at et; simp at et
---   rw[<-et];
---   generalize instsp : get_instances Γ n = ιs at et; symm at instsp
---   generalize tlp' : List.map (·.apply_spine sp) ιs = tl' at *; symm at tlp'
---   apply Red.ctor2_congr1
---   simp
---   apply Red.inst;
---   apply Eq.symm fnf
---   simp; unfold Frame.is_openm; rw[om]
---   apply instsp;
---   apply tlp'
---   rfl
+case _ => apply Red.ite_map
+case _ ih1 =>
+  rw[Option.bind_eq_some] at et;
+  cases et; case _ u1 et =>
+  cases et; case _ h1 et =>
+  cases et
+  replace h1 := ih1 h1
+  apply Red.ite_congr; assumption
 
--- case _ Γ f t _ n sp fnf A t' lt et => -- app term
---   simp at et; rw[fnf] at et; simp at et; rw[lt] at et; simp at et
---   rw[<-et]
---   apply Red.ctor2_congr1
---   simp
---   apply Red.letterm
---   apply Eq.symm fnf
---   apply Eq.symm lt
+case _ => apply Red.guard_map
+case _ ih1 =>
+  rw[Option.bind_eq_some] at et;
+  cases et; case _ u1 et =>
+  cases et; case _ h1 et =>
+  cases et
+  replace h1 := ih1 h1
+  apply Red.guard_congr; assumption
 
--- case _ et => -- app
---   simp at et; split at et;
---   case _ => simp_all
---   case _ => simp_all
+case _ => apply Red.ctor1_map
 
--- case _ Γ f t _ nf ih et =>
---   simp at et; simp_all;
---   rw[Option.bind_eq_some] at et
---   cases et; case _ w h =>
---     have ih' := @ih w (And.left h)
---     injection (And.right h) with ts; subst ts; simp at h;
---     apply Red.ctor2_congr1;
---     simp; assumption
+case _ ih1 ih2 =>
+  rw[Option.bind_eq_some] at et;
+  cases et; case _ u1 et =>
+  cases et; case _ h1 et =>
+  cases et
+  replace h2 := ih2 h1
+  apply Red.ctor1_congr; assumption
 
--- case _ Γ f t _ n sp fnf _ om et => -- appt openm
---   simp at et; rw[fnf] at et; simp at et; rw[om] at et; simp at et
---   rw[<-et];
---   generalize instsp : get_instances Γ n = ιs at et; symm at instsp
---   generalize tlp' : List.map (·.apply_spine sp) ιs = tl' at *; symm at tlp'
---   apply Red.ctor2_congr1
---   simp
---   apply Red.inst;
---   apply Eq.symm fnf
---   simp; unfold Frame.is_openm; rw[om]
---   apply instsp;
---   apply tlp'
---   rfl
+case _ => apply Red.ctor2_map2; simp; simp
 
--- case _ Γ f t _ n sp fnf A t' lt et => -- appt term
---   simp at et; rw[fnf] at et; simp at et; rw[lt] at et; simp at et
---   rw[<-et]
---   apply Red.ctor2_congr1
---   simp
---   apply Red.letterm
---   apply Eq.symm fnf
---   apply Eq.symm lt
+case _ => apply Red.ctor2_map2; simp; simp
 
--- case _ et =>
---   simp at et; split at et
---   case _ => simp_all
---   case _ => simp_all
+case _ => apply Red.ctor2_map2; simp; simp
 
--- case _ Γ f t _ nf ih et =>
---   simp at et; simp_all;
---   rw[Option.bind_eq_some] at et
---   cases et; case _ w h =>
---     have ih' := @ih w (And.left h)
---     injection (And.right h) with ts; subst ts;
---     simp at h
---     apply Red.ctor2_congr1; simp; assumption
+case _ h1 ih1 =>
+  simp_all; rw[<-et]; apply Red.ctor2_congr1; simp; assumption
 
--- -- ITE
--- case _ Γ p s b c ih et =>
---   simp at et;
---   rw[Option.bind_eq_some] at et;
---   cases et; case _ w h =>
---     have pne := And.left h;
---     have site := And.right h;
---     simp at site; split at site; simp_all;
---     case _ =>
---       rw[Option.bind_eq_some] at site;
---       cases site; case _ w h =>
---       cases h; case _ h =>
---       injection (And.right h) with ts; subst ts; simp at h;
---       apply Red.ite_congr (ih h)
---     case _ snf =>
---       simp_all;
---       have wisctor := site.1;
---       replace site := site.2;
---       split at site;
---       case _ => rw[Option.bind_eq_some] at site; cases site; case _ w h =>
---         simp at h;
---         have tl' := h.2;
---         subst tl';
---         apply Red.ite_congr (ih h.1)
---       case _ s'_stable =>
---         simp_all; split at site;
---         case _ headeqs =>
---           split at site;
---           case _ pfix =>
---             injection site with site; subst headeqs;
---             symm at snf; symm at pne; subst site; symm at pfix;
---             apply Red.ite_matched pne snf pfix wisctor;
---           case _ pfix =>
---              injection site with site; subst site; symm at snf; symm at pne;
---              have x :=  option_lemma pfix;
---              apply Red.ite_missed pne snf s'_stable (Or.inr x)
---         case _ h =>
---           injection site with site; subst site;
---           symm at snf; symm at pne;
---           apply Red.ite_missed pne snf s'_stable (Or.inl h)
+case _ h1 _ h2 ih1 ih2 =>
+  simp_all; rw[<-et]; apply Red.ctor2_congr2; simp; assumption
 
--- -- GUARD
--- case _ Γ p s c ih et =>
---   simp at et;
---   rw[Option.bind_eq_some] at et;
---   cases et; case _ w h =>
---   have pne := And.left h;
---   have smatch := And.right h;
---   simp_all; split at smatch;
---   case _ =>
---     rw[Option.bind_eq_some] at smatch;
---     cases smatch; case _ s' smatch' =>
---     cases smatch'; case _ smatch' =>
---     have ih' := ih (And.left smatch'); simp_all
---     have h' := And.right smatch'; subst h'; apply Red.guard_congr ih'
---   case _ s' sp' snf =>
---     split at smatch;
---     case _ frame_term =>
---       rw[Option.bind_eq_some] at smatch;
---       symm at snf; symm at frame_term; simp_all
---       cases smatch;
---       case _ w ts' =>
---         cases ts';
---         case _ ts' =>
---           have ih' := ih (And.left ts'); simp_all
---           have h' := And.right ts'; subst h'; apply Red.guard_congr ih'
---     case _ =>
---       simp_all; split at smatch;
---       case _ s'_stable s_n =>
---         subst s_n; have s_is_inst := smatch.1; replace smatch := smatch.2;
---         split at smatch;
---         case _ pfix =>
---              injection smatch with smatch; subst smatch;
---              symm at snf; symm at pne; symm at pfix;
---              apply Red.guard_matched pne snf pfix;
---         case _ pfix =>
---              injection smatch with smatch; subst smatch; symm at snf; symm at pne;
---              have x :=  option_lemma pfix;
---              apply Red.guard_missed pne snf s'_stable (Or.inr x)
---       case _ xx heq =>
---            have tl' := smatch.2; injection tl' with tl'; subst tl';
---            replace smatch := smatch.1;
---            symm at pne; symm at snf;
---            have reds : Red Γ (.guard p s c) `0 := (Red.guard_missed pne snf xx (Or.inl heq));
---            apply reds
+case _ h1 h2 _ _ => rw[h1] at et; rw[h2] at et; simp at et
 
--- case _ Γ _ et => simp at et; rw[<-et]; apply Red.sym
+case _ v _ _ _ _ _ _ _ _ _ _ h =>
+  cases et; case _ h1 et =>
+  have h' := @LawfulBEq.eq_of_beq Ctor2Variant _ _ v .choice h
+  subst h'; simp at h1
 
--- case _ ih et =>
---   simp at et; rw[Option.bind_eq_some] at et;
---   cases et; case _ w h =>
---   have et' := ih (And.left h); simp_all; rw[<-And.right h];
---   apply Red.ctor1_congr; assumption
+case _ v _ _ _ _ _ _ _ _ _ _ h0 h =>
+  cases et; case _ h1 et =>
+  cases et; case _ h2 et =>
+  simp at h; rw[h] at h2
+  rw[<-et]
+  apply Red.ctor2_map1
+  apply h
+  simp; simp at h0;
+  cases v;
+  all_goals (simp_all)
 
--- case _ Γ K t K' t' teq et =>
---   simp at teq
---   have e1 := Term.eq_of_beq teq.1; subst e1;
---   have e2 := Term.eq_of_beq teq.2; subst e2;
---   simp at et; rw [<-et]; exact Red.seq
+case _ v _ _ _ _ _ _ _ _ _ _ h =>
+  cases et; case _ h1 et =>
+  cases et; case _ h2 et =>
+  simp at h; rw[h] at h2; cases h2
 
--- case _ Γ K t t' K' h et =>
---   simp at et; have nh := And.left et; exfalso;
---   simp at h;
---   have e := h nh.1
---   have e' := nh.2; rw[e] at e'
---   contradiction
+case _ => apply Red.bind2_map1; simp
 
--- case _ ih1 ih2 et =>
---   simp at et;
---   rw[Option.bind_eq_some] at et;
---   cases et; case _ u et =>
---   have et1 := et.1
---   replace et := et.2;  injection et with et; subst et
---   have lem1 := ih2 et1;
---   apply Red.ctor2_congr2
---   simp; assumption
+case _ => apply Red.bind2_map2; simp
 
--- case _ Γ _ _  ih et =>
---   simp at et; rw[Option.bind_eq_some] at et;
---   cases et; case _ u et =>
---   have et1 := et.1
---   replace et := et.2;  injection et with et; subst et
---   have lem1 := ih et1
---   apply Red.ctor2_congr1
---   simp; assumption
 
--- case _ Γ K1 K t K2 t' e et =>
---   simp at et;
---   replace et := et.2; rw [<-et];
---   replace e := Term.eq_of_beq e; subst e
---   apply Red.appc
+theorem eval_const_folding1_soudness : eval_const_folding1 Γ t = .some t' -> Red Γ t t' := by
+intro et;
+induction Γ, t using eval_const_folding1.induct generalizing t'
+all_goals(simp at et)
+all_goals try (rw[<-et])
+all_goals try (
+case _ ih1 =>
+  rw[Option.bind_eq_some] at et;
+  cases et; case _ et =>
+  cases et; case _ h1 et =>
+  cases et;
+  replace h1 := ih1 h1
+  apply Red.bind2_congr2; simp; assumption
+)
+all_goals try (
+case _ ih1 =>
+  rw[Option.bind_eq_some] at et;
+  cases et; case _ et =>
+  cases et; case _ h1 et =>
+  cases et;
+  replace h1 := ih1 h1
+  apply Red.ctor2_congr2; simp; assumption
+)
 
--- case _ Γ K1 K t K2 t' e et =>
---   simp at et
---   have e1 := Term.eq_of_beq et.1
---   cases e1; simp at e
+case _ => apply Red.ite_absorb
+case _ ih1 =>
+  rw[Option.bind_eq_some] at et;
+  cases et; case _ et =>
+  cases et; case _ h1 et =>
+  cases et;
+  replace h1 := ih1 h1
+  apply Red.ite_congr; assumption
 
--- case _ ih et =>
---   simp at et; rw[Option.bind_eq_some] at et;
---   cases et; case _ u et =>
---   have et1 := et.1
---   replace et := et.2;  injection et with et; subst et
---   have lem1 := ih et1;
---   apply Red.ctor2_congr2; simp; assumption
+case _ => apply Red.guard_absorb
+case _ ih1 =>
+  rw[Option.bind_eq_some] at et;
+  cases et; case _ et =>
+  cases et; case _ h1 et =>
+  cases et;
+  replace h1 := ih1 h1
+  apply Red.guard_congr; assumption
 
--- case _ ih et =>
---   simp at et; rw[Option.bind_eq_some] at et;
---   cases et; case _ u et =>
---   have et1 := et.1
---   replace et := et.2;  injection et with et; subst et
---   have lem1 := ih et1;
---   apply Red.ctor2_congr1; simp; assumption
+case _ => apply Red.ctor1_absorb
+case _ ih1 =>
+  rw[Option.bind_eq_some] at et;
+  cases et; case _ et =>
+  cases et; case _ h1 et =>
+  cases et;
+  replace h1 := ih1 h1
+  apply Red.ctor1_congr; assumption
 
--- case _ et => simp at et; subst et; apply Red.fst
+case _ => apply Red.choice1
+case _ => apply Red.choice2
+case _ => apply Red.ctor2_absorb2; simp
 
--- case _ ih et =>
---   simp at et; rw[Option.bind_eq_some] at et;
---   cases et; case _ u et =>
---   have et1 := et.1
---   replace et := et.2;  injection et with et; subst et
---   have lem1 := ih et1;
---   apply Red.ctor2_congr2; simp; assumption
+case _ => apply Red.ctor2_absorb2; simp
 
--- case _ et => simp at et; subst et; apply Red.snd
--- case _ ih et =>
---   simp at et; rw[Option.bind_eq_some] at et;
---   cases et; case _ u et =>
---   have et1 := et.1
---   replace et := et.2;  injection et with et; subst et
---   have lem1 := ih et1;
---   apply Red.ctor2_congr2; simp; assumption
+case _ => apply Red.ctor2_absorb2; simp
 
--- case _ et => -- arrowc
---  simp at et; subst et; apply Red.arrowc
--- case _ ih et =>
---  simp at et; rw[Option.bind_eq_some] at et;
---  cases et; case _ η' h =>
---  have ih' := @ih η' h.1;
---  injection h.2 with w; subst w
---  apply Red.bind2_congr2; simp; assumption
--- case _ Γ η η' ih ih1 ih2 et =>
---  simp at et; rw[Option.bind_eq_some] at et;
---  cases et; case _ η1' h =>
---  have ih' := @ih2 η1' h.1;
---  injection h.2 with w; subst w; simp at h;
---  apply Red.bind2_congr1; simp; assumption
+case _ v _ _ _ _ _ _ _ _ h =>
+  cases et; case _ h2 et =>
+  simp at h; rw[h] at h2
+  rw[<-et]
+  apply Red.ctor2_absorb1
+  assumption
 
--- case _ et => -- allc
---  simp at et; subst et; apply Red.allc
--- case _ ih et =>
---  simp at et; rw[Option.bind_eq_some] at et;
---  cases et; case _ η1' h =>
---  have ih' := @ih η1' h.1;
---  injection h.2 with w; subst w; simp at h;
---  apply Red.bind2_congr2; simp; assumption
+case _ v _ _ _ _ _ _ _ _ _ _ =>
+  cases et; case _ h1 et =>
+  rw[<-et]
+  apply @Red.ctor2_absorb1 v;
+  assumption
 
--- case _ et => -- apptc
---  simp at et; have e1 := Term.eq_of_beq et.1; subst e1;
---  replace et := et.2; subst et
---  apply Red.apptc
--- case _ e et =>
---  simp at et; have e1 := Term.eq_of_beq et.1; subst e1
---  simp at e
--- case _ ih et =>
---  simp at et; rw[Option.bind_eq_some] at et;
---  cases et; case _ u et =>
---  have et1 := et.1
---  replace et := et.2;  injection et with et; subst et
---  have lem1 := ih et1;
---  apply Red.ctor2_congr1; simp; assumption
--- case _ ih et =>
---  simp at et; rw[Option.bind_eq_some] at et;
---  cases et; case _ u et =>
---  have et1 := et.1
---  replace et := et.2;  injection et with et; subst et
---  have lem1 := ih et1;
---  apply Red.ctor2_congr2; simp; assumption
+case _ h1 ih1 =>
+  rw[h1] at et; simp at et; rw[<-et];
+  replace h1 := ih1 h1
+  apply Red.ctor2_congr1; simp; assumption
+case _ h1 _ h2 ih1 ih2 =>
+  rw[h1] at et; rw[h2] at et; simp at et; rw[<-et]
+  replace h2 := ih2 h2
+  apply Red.ctor2_congr2; simp; assumption
+case _ h1 h2 _ _ => rw[h1] at et; rw[h2] at et; simp at et
+case _ h1 _ h2 ih1 =>
+  simp_all
+  rw[<-et]
+  apply Red.ctor2_congr1; assumption; assumption
+case _ h1 h2 h3 h4 _ h5 ih1 ih2 =>
+  simp_all
+  rw[<-et]
+  apply Red.ctor2_congr2; assumption; assumption
+case _ => simp_all
+case _ => simp_all
+case _ =>
+  simp_all
+  rw[<-et]
+  apply Red.ctor2_congr2; assumption; assumption
+case _ => simp_all
+case _ => simp_all
+case _ => apply @Red.bind2_absorb1 .arrowc; simp
+case _ => apply @Red.bind2_absorb2 .allc; simp
 
--- case _ Γ t a ih => -- cast
---   simp at ih; rw[<-ih]; exact Red.cast
--- case _ Γ t η x ih1 ih=>
---   simp at ih; rw[Option.bind_eq_some] at ih;
---   cases ih; case _ h w =>
---   have h' := w.2; injection h' with w';
---   have qq := @ih1 h w.1
---   rw [<-w'];
---   apply Red.ctor2_congr2; simp; assumption
+theorem eval_const_folding2_soudness : eval_const_folding2 Γ t = .some t' -> Red Γ t t' := by
+intro et;
+induction Γ, t using eval_const_folding2.induct generalizing t'
+all_goals(simp at et)
+all_goals try (rw[<-et])
+all_goals try (
+case _ ih1 =>
+  rw[Option.bind_eq_some] at et;
+  cases et; case _ et =>
+  cases et; case _ h1 et =>
+  cases et;
+  replace h1 := ih1 h1
+  apply Red.bind2_congr2; simp; assumption
+)
+all_goals try (
+case _ ih1 =>
+  rw[Option.bind_eq_some] at et;
+  cases et; case _ et =>
+  cases et; case _ h1 et =>
+  cases et;
+  replace h1 := ih1 h1
+  apply Red.ctor2_congr2; simp; assumption
+)
+all_goals try (
+case _ ih1 =>
+  rw[Option.bind_eq_some] at et;
+  cases et; case _ et =>
+  cases et; case _ h1 et =>
+  cases et;
+  replace h1 := ih1 h1
+  apply Red.ctor1_congr; assumption
+)
 
--- case _ et => simp at et -- zero
+case _ ih1 =>
+  rw[Option.bind_eq_some] at et;
+  cases et; case _ et =>
+  cases et; case _ h1 et =>
+  cases et;
+  replace h1 := ih1 h1
+  apply Red.ite_congr; assumption
 
--- case _ et => -- choice
---   simp at et; subst et; constructor
--- case _ et =>
---  simp at et; subst et; constructor
--- case _ h ih1 et =>
---   simp at et; rw[h] at et; simp at et; rw[<-et]
---   have ih' := ih1 h
---   apply Red.ctor2_congr1; simp; assumption
--- case _ h1 _ h2 _ ih et =>
---   simp at et; rw[h1] at et; simp at et; rw[h2] at et; simp at et
---   rw[<-et]
---   have ih' := ih h2
---   apply Red.ctor2_congr2; simp; assumption
--- case _ h1 h2 _ _ et =>
---   simp at et; rw[h1] at et; simp at et; rw[h2] at et; simp at et
--- case _ et => simp at et
+case _ ih1 =>
+  rw[Option.bind_eq_some] at et;
+  cases et; case _ et =>
+  cases et; case _ h1 et =>
+  cases et;
+  replace h1 := ih1 h1
+  apply Red.guard_congr; assumption
+
+case _ v _ _ => cases v; apply Red.sym;
+
+case _ => apply Red.cast
+
+case _ => apply Red.fst
+
+case _ => apply Red.snd
+
+case _ h =>
+  simp at h;
+  have e1 := Term.eq_of_beq h.1
+  have e2 := Term.eq_of_beq h.2
+  rw[<-et.2]; subst e1; subst e2
+  apply Red.seq
+case _ h =>
+  simp at h
+  exfalso; have h' := h et.1.1
+  have e := et.1.2; rw[h'] at e; simp at e
+
+case _ h =>
+  replace h := Term.eq_of_beq h
+  have h1 := Term.eq_of_beq et.1
+  cases et; case _ et =>
+  cases h1;
+  rw[<-et]
+  apply Red.appc
+case _ h =>
+  replace h := Term.eq_of_beq et.1
+  have h1 := Term.eq_of_beq et.1
+  rw[<-et.2];
+  cases h1;
+  apply Red.appc
+
+case _ =>
+  replace h := Term.eq_of_beq et.1
+  have h1 := Term.eq_of_beq et.1
+  rw[<-et.2];
+  cases h1;
+  apply Red.apptc
+
+case _ =>
+  have h := Term.eq_of_beq et.1; cases h; simp_all
+
+case _ h1 ih1 =>
+  rw[h1] at et; simp at et; rw[<-et];
+  replace h1 := ih1 h1
+  apply Red.ctor2_congr1; simp; assumption
+
+case _ h1 _ h2 ih1 ih2 =>
+  rw[h1] at et; rw[h2] at et; simp at et; rw[<-et]
+  replace h2 := ih2 h2
+  apply Red.ctor2_congr2; simp; assumption
+
+case _ h1 h2 _ _ => rw[h1] at et; rw[h2] at et; simp at et
+
+case _ h ih1 => simp_all; rw[<-et]; apply Red.ctor2_congr1; assumption; assumption
+
+case _ h1 h2 ih1 => simp_all; rw[<-et]; apply Red.ctor2_congr2; assumption; assumption
+
+case _ => simp_all
+
+case _ => simp_all
+case _ => simp_all; rw[<-et]; apply Red.ctor2_congr2; assumption; assumption
+case _ => simp_all
+case _ => simp_all
+
+case _ => apply Red.arrowc
+case _ => apply Red.allc
+
+
+theorem eval_inst_soundess : eval_inst Γ t = .some t' -> Red Γ t t' := by
+intro et;
+induction Γ, t using eval_inst.induct generalizing t'
+all_goals (simp at et)
+all_goals try (rw[<-et])
+
+all_goals try (
+case _ ih1 =>
+  rw[Option.bind_eq_some] at et;
+  cases et; case _ et =>
+  cases et; case _ h1 et =>
+  cases et;
+  replace h1 := ih1 h1
+  apply Red.ctor1_congr; assumption
+)
+
+all_goals try (
+case _ ih1 =>
+  rw[Option.bind_eq_some] at et;
+  cases et; case _ t' et =>
+  cases et; case _ h1 et =>
+  cases et
+  replace h1 := ih1 h1
+  apply Red.ctor2_congr1; simp; assumption
+)
+
+all_goals try (
+case _ ih1 =>
+  rw[Option.bind_eq_some] at et;
+  cases et; case _ et =>
+  cases et; case _ h1 et =>
+  cases et;
+  replace h1 := ih1 h1
+  apply Red.ctor2_congr2; simp; assumption
+)
+
+all_goals try (
+case _ ih1 =>
+  rw[Option.bind_eq_some] at et;
+  cases et; case _ t' et =>
+  cases et; case _ h1 et =>
+  cases et
+  replace h1 := ih1 h1
+  apply Red.bind2_congr2; simp; assumption
+)
+
+all_goals try (
+case _ ih1 =>
+  rw[Option.bind_eq_some] at et;
+  cases et; case _ t' et =>
+  cases et; case _ h1 et =>
+  cases et
+  replace h1 := ih1 h1
+  apply Red.bind2_congr1; simp; assumption
+)
+
+case _ Γ n _ om =>
+  simp_all; subst et;
+  generalize instsp : get_instances Γ n = insts at *;
+  have nfh := @Term.var_neutral_form n; symm at nfh;
+  symm at instsp;
+  apply Red.inst nfh _ instsp; unfold Term.apply_spine; simp_all;
+  apply instsp; rfl
+  simp; rw[om]; unfold Frame.is_openm; simp
+case _ Γ n _ _ lt =>
+    rw [lt] at et; simp at et; subst et;
+    have nf :=  @Term.var_neutral_form n; symm at nf; symm at lt;
+    apply Red.letterm nf lt;
+case _ => apply Red.letbeta
+case _ Γ p s b c ih =>
+  rw[Option.bind_eq_some] at et;
+  cases et; case _ w h =>
+    have pne := And.left h;
+    have site := And.right h;
+    simp at site; split at site; simp_all;
+    case _ =>
+      rw[Option.bind_eq_some] at site;
+      cases site; case _ w h =>
+      cases h; case _ h =>
+      injection (And.right h) with ts; subst ts; simp at h;
+      apply Red.ite_congr (ih h)
+    case _ snf =>
+      simp_all;
+      have wisctor := site.1;
+      replace site := site.2;
+      split at site;
+      case _ => rw[Option.bind_eq_some] at site; cases site; case _ w h =>
+        simp at h;
+        have tl' := h.2;
+        subst tl';
+        apply Red.ite_congr (ih h.1)
+      case _ s'_stable =>
+        simp_all; split at site;
+        case _ headeqs =>
+          split at site;
+          case _ pfix =>
+            injection site with site; subst headeqs;
+            symm at snf; symm at pne; subst site; symm at pfix;
+            apply Red.ite_matched pne snf pfix wisctor;
+          case _ pfix =>
+             injection site with site; subst site; symm at snf; symm at pne;
+             have x :=  option_lemma pfix;
+             apply Red.ite_missed pne snf s'_stable (Or.inr x)
+        case _ h =>
+          injection site with site; subst site;
+          symm at snf; symm at pne;
+          apply Red.ite_missed pne snf s'_stable (Or.inl h)
+
+case _ Γ p s c ih =>
+  rw[Option.bind_eq_some] at et;
+  cases et; case _ w h =>
+  have pne := And.left h;
+  have smatch := And.right h;
+  simp_all; split at smatch;
+  case _ =>
+    rw[Option.bind_eq_some] at smatch;
+    cases smatch; case _ s' smatch' =>
+    cases smatch'; case _ smatch' =>
+    have ih' := ih (And.left smatch'); simp_all
+    have h' := And.right smatch'; subst h'; apply Red.guard_congr ih'
+  case _ s' sp' snf =>
+    split at smatch;
+    case _ frame_term =>
+      rw[Option.bind_eq_some] at smatch;
+      symm at snf; symm at frame_term; simp_all
+      cases smatch;
+      case _ w ts' =>
+        cases ts';
+        case _ ts' =>
+          have ih' := ih (And.left ts'); simp_all
+          have h' := And.right ts'; subst h'; apply Red.guard_congr ih'
+    case _ =>
+      simp_all; split at smatch;
+      case _ s'_stable s_n =>
+        subst s_n; have s_is_inst := smatch.1; replace smatch := smatch.2;
+        split at smatch;
+        case _ pfix =>
+             injection smatch with smatch; subst smatch;
+             symm at snf; symm at pne; symm at pfix;
+             apply Red.guard_matched pne snf pfix;
+        case _ pfix =>
+             injection smatch with smatch; subst smatch; symm at snf; symm at pne;
+             have x :=  option_lemma pfix;
+             apply Red.guard_missed pne snf s'_stable (Or.inr x)
+      case _ xx heq =>
+           have tl' := smatch.2; injection tl' with tl'; subst tl';
+           replace smatch := smatch.1;
+           symm at pne; symm at snf;
+           have reds : Red Γ (.guard p s c) `0 := (Red.guard_missed pne snf xx (Or.inl heq));
+           apply reds
+
+case _ => apply Red.beta
+
+case _ n _ tnf ih1 => -- app recursive case
+  rw[tnf] at et; simp at et;
+  rw[Option.bind_eq_some] at et;
+  cases et; case _ t' et =>
+  cases et; case _ h1 et =>
+  cases et
+  replace h1 := ih1 h1
+  apply Red.ctor2_congr1; simp; assumption
+
+case _ Γ f t e n sp fnf t' om => -- app openm
+  rw[fnf] at et; simp at et; rw[om] at et; simp at et
+  rw[<-et];
+  generalize instsp : get_instances Γ n = ιs at et; symm at instsp
+  generalize tlp' : List.map (·.apply_spine sp) ιs = tl' at *; symm at tlp'
+  apply Red.ctor2_congr1
+  simp
+  apply Red.inst;
+  apply Eq.symm fnf
+  simp; unfold Frame.is_openm; rw[om]
+  apply instsp;
+  apply tlp'
+  rfl
+
+case _ n _ tnf _ _ lt => -- app let term
+  rw[tnf] at et; simp at et;
+  rw [lt] at et; simp at et; subst et;
+  apply Red.ctor2_congr1; simp;
+  symm at tnf; symm at lt;
+  apply Red.letterm; assumption; assumption
+
+case _ n _ tnf _ _ => -- app bogus
+  rw[tnf] at et; simp at et;
+
+
+case _ => apply Red.betat
+case _ Γ f t e n sp fnf t' om =>  -- appt openm
+  rw[fnf] at et; simp at et; rw[om] at et; simp at et
+  rw[<-et];
+  generalize instsp : get_instances Γ n = ιs at et; symm at instsp
+  generalize tlp' : List.map (·.apply_spine sp) ιs = tl' at *; symm at tlp'
+  apply Red.ctor2_congr1
+  simp
+  apply Red.inst;
+  apply Eq.symm fnf
+  simp; unfold Frame.is_openm; rw[om]
+  apply instsp;
+  apply tlp'
+  rfl
+
+case _ n _ tnf _ _ lt => -- appt let term
+  rw[tnf] at et; simp at et;
+  rw [lt] at et; simp at et; subst et;
+  apply Red.ctor2_congr1; simp;
+  symm at tnf; symm at lt;
+  apply Red.letterm; assumption; assumption
+
+case _ n _ tnf _ _ => -- appt bogus
+  rw[tnf] at et; simp at et;
+
+case _ n _ tnf ih1 => -- appt recursive case
+  rw[tnf] at et; simp at et;
+  rw[Option.bind_eq_some] at et;
+  cases et; case _ t' et =>
+  cases et; case _ h1 et =>
+  cases et
+  replace h1 := ih1 h1
+  apply Red.ctor2_congr1; simp; assumption
+
+case _ h0 _ h1 ih1 =>
+ rw[h1] at et; simp at et;
+ replace h1 := ih1 h1
+ simp at h0; rw[h0] at et; simp at et
+ rw[<-et]
+ apply Red.ctor2_congr1; assumption; assumption
+
+case _ h1 h2 h3 _ h4 ih1 ih2 =>
+  simp at h1; simp at h3; rw[h1] at et; rw[h4] at et; rw[h2] at et; simp at et
+  cases et; case _ et =>
+  replace h4 := ih2 h4
+  rw[<-et]
+  apply Red.ctor2_congr2; assumption; assumption
+
+case _ h1 h2 h3 h4 _ _ => rw[h2] at et; rw[h4] at et; simp at et
+
+case _ h1 h2 h3 ih1 =>
+  simp at h1; rw[h1] at et;
+  rw[h2] at et; simp at et
+  cases et; case _ h4 et =>
+  simp at h3;
+  simp_all
+
+case _ h1 h2 h3 h4 ih1 =>
+  simp_all
+  rw[<-et]
+  apply Red.ctor2_congr2; assumption; assumption
+case _ =>  simp_all
+
+case _ => simp_all
+
+
+theorem eval_small_step_soundness : eval_small_step Γ t = some t' -> Red Γ t t' := by
+intro et; unfold eval_small_step at et
+split at et
+case _ =>
+ cases et; case _ et =>
+ apply eval_choice_mapping_soudness et
+case _ e =>
+  split at et
+  case _ =>
+    cases et; case _ et =>
+    apply eval_const_folding1_soudness et
+  case _ =>
+    split at et
+    case _ =>
+      cases et; case _ et =>
+      apply eval_const_folding2_soudness et
+    case _ =>
+      split at et
+      case _ =>
+        cases et; case _ et =>
+        apply eval_inst_soundess et
+      cases et
