SystemFD/Examples/SuperClasses.lean
@@ -13,7 +13,7 @@ def OrdEqBoolCtx : Ctx Term := [
      -/
      .inst #5 (Λ[★] `λ[#7 `@k #0]
        Term.guard (#5 `@t #1) #0 (`λ[#1 ~[★]~ #16]
-         (`λ[#17] `λ[#18] (#6 `@ (#5 `@ #1) `@ #0)) ▹ ((sym! #0) -c> ((sym! #1) -c> refl! ★ #19))
+         ((`λ[#17] `λ[#18] (#6 `@ (#5 `@ #1) `@ #0)) ▹ ((sym! #0) -c> ((sym! #1) -c> (refl! ★ #19))))
        )),
 
     -- not : Bool → Bool
@@ -58,3 +58,36 @@ def leq := Λ[★] `λ[#8 `@k #0] `λ[#1] `λ[#2] (
 #eval infer_type OrdEqBoolCtx leq
 #eval eval_ctx_loop OrdEqBoolCtx (leq `@t #15 `@ (#4 `@t #15 `@ (refl! ★ #15)) `@ #13 `@ #14)
 #eval eval_ctx_loop OrdEqBoolCtx (leq `@t #15 `@ (#4 `@t #15 `@ (refl! ★ #15)) `@ #14 `@ #13)
+
+
+#eval infer_type OrdEqBoolCtx
+      ((sym! (refl! ★ #15)) -c> (sym! (refl! ★ #16)) -c> (refl! ★ #17))
+
+#eval infer_type OrdEqBoolCtx
+      ((sym! (refl! ★ (#15 -t> #16 -t> #17))))
+
+
+#eval infer_type OrdEqBoolCtx
+      (((`λ[#15] (`λ[#16]
+          (((#4 `@  (#3 `@ #1)) `@  #0)
+            ▹ ((sym! (refl! ★ #17)) -c> (sym! (refl! ★ #18)) -c> (refl! ★ #19))
+            -- ▹ ((sym! (refl! ★ (#17 -t> #18 -t> #19))))
+           ))
+          `@ #13)
+          `@ #14
+          ))
+
+
+#eval eval_ctx_loop OrdEqBoolCtx
+      (((`λ[#15] (`λ[#16]
+          (((#4 `@  (#3 `@ #1)) `@  #0)
+            -- ▹ (sym! (refl! ★ #15)) -c> (sym! (refl! ★ #16)) -c> (refl! ★ #17)
+            )))
+          `@ #13)
+          `@ #14
+          )
+
+-- #eval eval_ctx_loop OrdEqBoolCtx
+--       (`λ[#15] `λ[#16]
+--           ((#4 `@  (#3 `@ #1)) `@  #0) ▹
+--           (sym! (refl! ★ #15)) -c> (sym! (refl! ★ #16)) -c> (refl! ★ #17)) `@  #13 `@ #14
